SP1Operations/Compare/IsEqualWordOperation.lean
@@ -2,12 +2,23 @@ import SP1Operations.Compare.IsEqualWordOperation.Constraints
 
 namespace IsEqualWordOperation
 
+attribute [local simp ← high] Word.eq_pointwise
+
 @[grind →, aesop safe forward]
 lemma spec
   {a b : Word (Fin BB)}
   {cols : IsEqualWordOperation} :
   List.Forall SP1Constraint.toProp (constraints a b cols 1) →
     cols.is_diff_zero.result = if a = b then 1 else 0
+  := by simp [constraints]; grind
+
+lemma spec.gen
+  {a b : Word (Fin BB)}
+  {cols : IsEqualWordOperation}
+  {is_real : Fin BB} :
+  List.Forall SP1Constraint.toProp (constraints a b cols is_real) →
+    is_real = (1 : Fin BB) →
+      cols.is_diff_zero.result = if a = b then 1 else 0
   := by simp [constraints]; grind
 
 end IsEqualWordOperation
