SP1Operations/Compare/IsZeroWordOperation.lean
@@ -2,7 +2,7 @@ import SP1Operations.Compare.IsZeroWordOperation.Constraints
 
 namespace IsZeroWordOperation
 
-attribute [simp ← high] Word.eq_pointwise
+attribute [local simp ← high] Word.eq_pointwise
 
 @[grind →, aesop safe forward]
 lemma spec
@@ -10,6 +10,15 @@ lemma spec
   {cols : IsZeroWordOperation} :
   List.Forall SP1Constraint.toProp (constraints a cols 1) →
     cols.result = if a = #v[(0 : Fin BB), (0 : Fin BB), (0 : Fin BB), (0 : Fin BB)] then 1 else 0
+  := by simp [constraints]; grind
+
+lemma spec.gen
+  {a : Word (Fin BB)}
+  {cols : IsZeroWordOperation}
+  {is_real : Fin BB}:
+  List.Forall SP1Constraint.toProp (constraints a cols is_real) →
+    is_real = 1 →
+      cols.result = if a = #v[(0 : Fin BB), (0 : Fin BB), (0 : Fin BB), (0 : Fin BB)] then 1 else 0
   := by simp [constraints]; grind
 
 end IsZeroWordOperation
